verif/Kinit_eval.v
@@ -1,0 +1,122 @@
+Require Import List.
+Import ListNotations.
+Require Import String.
+
+(* Borrow from CompCert *)
+Require Import Coqlib.
+Require Import Bitvectors.
+
+Require Import AST.
+Require Import Semantics.
+Require Import Utils.
+Require Import Builtins.
+Require Import BuiltinSem.
+Require Import BuiltinSyntax.
+Require Import Values.        
+Require Import Eager.
+Require Import Bitstream.
+
+Require Import EvalTac.
+
+Import HaskellListNotations.
+Open Scope string.
+
+Require Import HMAC.
+
+Require Import HMAC_spec.
+
+(* Require Import Bvector.*)
+
+
+(* Eager tactics *)
+(* TODO: standardize *)
+Ltac ec := econstructor; try unfold mb; try reflexivity.
+Ltac fg := eapply eager_eval_global_var; [ reflexivity | eassumption | idtac].
+Ltac g := eapply eager_eval_global_var; try eassumption; try reflexivity.
+
+
+Ltac e :=
+  match goal with
+  | [ |- eager_eval_expr ?GE _ ?E (EVar ?id) _ ] =>
+    (try fg); (try reflexivity);
+    (try solve [eapply eager_eval_local_var; reflexivity]);
+    fail 1 "couldn't figure out variable"
+  | [ |- _ ] => ec
+  end.
+
+Definition typenum (n : Z) : Expr := ETyp (TCon (TC (TCNum n)) []).
+Definition pwBytes := typenum 64.
+Definition blockLength := typenum 64.
+Definition digest := typenum 0.
+
+
+Lemma kinit_eval :
+  forall k,
+    n_bits 64 k ->
+    forall h,
+      (exists hv,
+          eager_eval_expr ge tempty sempty h hv) ->
+    exists v,
+      eager_eval_expr ge tempty sempty (apply (tapply (EVar kinit) (pwBytes :: blockLength :: digest ::  nil)) (h :: (EList (map EValue k)) :: nil)) v /\ eager_eval_expr ge tempty sempty (EList (map EValue k)) v.
+Proof.
+  init_globals ge.
+  intros.
+  remember H as Hnb; clear HeqHnb.
+  eapply n_bits_eval in H; eauto.
+  destruct H. instantiate (3 := ge) in H.
+  instantiate (1 := sempty) in H.
+  instantiate (1 := tempty) in H.
+  destruct H.
+  inversion H. subst.
+  destruct H0.
+  eexists. split; try eassumption. unfold apply.
+  
+  e. e.
+  e. e. e.
+  
+  g.
+  e. e. repeat e.
+  e. repeat e.
+  e. repeat e.
+  eassumption.
+  e. 
+  eassumption.
+  e. e. e. e. g. e. repeat e.
+  e. e. e. g. e.
+  repeat e. repeat e.
+  simpl. repeat e.
+  simpl. e. repeat e.
+  repeat e. repeat e. 
+  
+
+  
+  e. e. e. fg. repeat e.
+  e. repeat e. e. repeat e. repeat e.
+  repeat e. repeat e.
+  simpl.
+
+  e. e. e. e. g.
+  repeat e. repeat e.
+  e. repeat e.
+  e. repeat e.
+  e. e. e. e. e. e. g.
+  repeat e. e. e. repeat e.
+  e. repeat e. e. e. e. e. g.
+  repeat e. repeat e.
+  repeat e. repeat e.
+
+  rewrite append_strict_list. reflexivity.  
+  
+  e. g. e. g.
+  e. e. e. e. g.
+  all: try solve [repeat e].
+  e. repeat e. repeat e.
+
+
+  replace (tnum 64) with (tnum (Z.of_nat (Datatypes.length x))).
+  rewrite splitAt_len. reflexivity.
+  
+  f_equal. omega.
+  simpl. reflexivity.
+
+Qed.
